pcuic/theories/PCUICAstUtils.v
@@ -301,16 +301,6 @@ Qed.
 
 Hint Rewrite context_assumptions_map context_assumptions_mapi : len.
 
-Lemma mapi_rec_compose {A B C} (g : nat -> B -> C) (f : nat -> A -> B) k l :
-  mapi_rec g (mapi_rec f l k) k = mapi_rec (fun k x => g k (f k x)) l k.
-Proof.
-  induction l in k |- *; simpl; auto. now rewrite IHl.
-Qed.
-
-Lemma mapi_compose {A B C} (g : nat -> B -> C) (f : nat -> A -> B) l :
-  mapi g (mapi f l) = mapi (fun k x => g k (f k x)) l.
-Proof. apply mapi_rec_compose. Qed.
-
 Lemma compose_map_decl f g x : map_decl f (map_decl g x) = map_decl (f ∘ g) x.
 Proof.
   destruct x as [? [?|] ?]; reflexivity.
